\documentclass[main.tex]{subfiles}

\begin{document}

\subproblem{}\label{2c}
\[A \subset B \land A \subset C \iff A \subset (B \cap C)\]
\begin{thm}[\ref{2c} holds]
	\(A \subset B \land A \subset C \iff A \subset (B \cap C)\)
\end{thm}
\begin{proof}
	To demonstrate double implication, it is sufficient to demonstrate each
	implication.

	\medskip{}
	First, consider \(A \subset B \land A \subset C\). Now suppose
	\(\neg [A \subset (B \cap C)]\). By the definition of the subset
	relation, we have that
	\(\neg (x \in A \implies [x \in (B \cap C)])\). By the definition of
	set intersection, we have that
	\(\neg (x \in A \implies [x \in B \land x \in C])\). By DeMorgan's Law,
	we have that \(x \in A \land (x \notin B \lor x \notin C)\). By the
	distribution of \(\land\) over \(\lor\), we have
	\((x \in A \land x \notin B) \lor (x \in A \land x \notin C)\). By
	DeMorgan's Law, we have that
	\(\neg (x \in A \implies x \in B) \lor \neg (x \in A \implies x \in B)\).
	By the definition of the subset relation, we have that
	\(\neg (A \subset B) \lor \neg (A \subset C)\). However,
	\(\neg (A \subset B)\) contradicts our assumption that \(A \subset B\),
	and \(\neg (A \subset C)\) contradicts our assumption that
	\(A \subset C\). Since both cases of the conditional result in
	contradiction, the conditional as a whole also contradicts our
	assumptions. So our supposition was false, and \(A \subset (B \cap C)\).
	Thus \(A \subset B \land A \subset C \implies A \subset (B \cap C)\).

	\medskip{}
	Second, consider \(A \subset (B \cap C)\). By the definition of the
	subset relation, we see \(x \in A \implies x \in (B \cap C)\). By the
	definition of set intersection, we have
	\(x \in A \implies (x \in B \land x \in C)\). By the distribution of
	\(\lor\) over \(\land\), we have
	\((x \in A \implies x \in B) \land (x \in A \implies x \in C)\). By the
	definition of the subset relation, we have that
	\(A \subset B \land A \subset C\). Thus
	\(A \subset (B \cap C) \implies A \subset B \land A \subset C\).

	\medskip{}
	Therefore, since both implications have been shown, it is certain that
	\(A \subset B \land A \subset C \iff A \subset (B \cap C)\).
\end{proof}


\end{document}

